zoo_saturn/inf_mpmc_queue_2: Introduce specifications and assertions.

theories/zoo_saturn/inf_mpmc_queue_2.v
@@ -1,5 +1,24 @@
 From zoo Require Import
   prelude.
+From zoo.common Require Import
+  countable.
+From zoo.iris.base_logic Require Import
+  lib.auth_nat_max
+  lib.twins
+  lib.auth_mono
+  lib.mono_list
+  lib.saved_pred
+  lib.oneshot.
+From zoo.language Require Import
+  notations.
+From zoo.program_logic Require Import
+  identifier
+  wise_prophets.
+From zoo.diaframe Require Import
+  diaframe.
+From zoo_std Require Import
+  optional
+  inf_array.
 From zoo_saturn Require Export
   base
   inf_mpmc_queue_2__code.
@@ -8,8 +27,375 @@ From zoo_saturn Require Import
 From zoo Require Import
   options.
 
+Section oflatten.
+  Definition oflatten `(l : list $ option A) :=
+    omap id l.
+End oflatten.
+
+Implicit Types l : location.
+Implicit Types front back : nat.
+Implicit Types v t : val.
+Implicit Types vs : list val.
+Implicit Types hist : list (option val).
+Implicit Types slot : optional val.
+Implicit Types slots : nat → optional val.
+Implicit Types η : gname.
+Implicit Types ηs : list gname.
+
+#[local] Program Definition prophet := {|
+  typed_prophet_type :=
+    identifier ;
+  typed_prophet_of_val v :=
+    match v with
+    | ValId id =>
+        Some id
+    | _ =>
+        None
+    end ;
+  typed_prophet_to_val id :=
+    #id ;
+|}.
+Solve Obligations of prophet with
+  try done.
+Next Obligation.
+  naive_solver.
+Qed.
+Implicit Types pasts prophss : nat → list prophet.(typed_prophet_type).
+
+Inductive lstate :=
+  | Producer
+  | ProducerProducer
+  | ProducerConsumer
+  | Consumer
+  | ConsumerProducer η
+  | ConsumerConsumer.
+#[local] Canonical lstate_O :=
+  leibnizO lstate.
+Implicit Types lstate : lstate.
+Implicit Types lstates : list lstate.
+
+Inductive lstep : lstate → lstate → Prop :=
+  | lstep_producer_producer :
+      lstep Producer ProducerProducer
+  | lstep_producer_consumer :
+      lstep Producer ProducerConsumer
+  | lstep_consumer_producer η :
+      lstep Consumer (ConsumerProducer η)
+  | lstep_consumer_consumer :
+      lstep Consumer ConsumerConsumer.
+
+Class InfMpmcQueue2G Σ `{zoo_G : !ZooG Σ} := {
+  #[local] inf_mpmc_queue_2_G_inf_array_G :: InfArrayG Σ ;
+  #[local] inf_mpmc_queue_2_G_prophets_G :: WiseProphetsG Σ prophet ;
+  #[local] inf_mpmc_queue_2_G_front_G :: AuthNatMaxG Σ ;
+  #[local] inf_mpmc_queue_2_G_model_G :: TwinsG Σ (leibnizO (list val)) ;
+  #[local] inf_mpmc_queue_2_G_history_G :: MonoListG Σ (option val) ;
+  #[local] inf_mpmc_queue_2_G_lstate_G :: AuthMonoG Σ lstep ;
+  #[local] inf_mpmc_queue_2_G_lstates_G :: MonoListG Σ gname ;
+  #[local] inf_mpmc_queue_2_G_saved_pred_G :: SavedPredG Σ val ;
+  #[local] inf_mpmc_queue_2_G_producer_G :: OneshotG Σ () () ;
+  #[local] inf_mpmc_queue_2_G_producers_G :: MonoListG Σ gname ;
+  #[local] inf_mpmc_queue_2_G_consumer_G :: OneshotG Σ () () ;
+  #[local] inf_mpmc_queue_2_G_consumers_G :: MonoListG Σ gname ;
+}.
+
+Definition inf_mpmc_queue_2_Σ := #[
+  inf_array_Σ ;
+  wise_prophets_Σ prophet ;
+  auth_nat_max_Σ ;
+  twins_Σ (leibnizO (list val)) ;
+  mono_list_Σ (option val) ;
+  mono_list_Σ gname ;
+  auth_mono_Σ lstep ;
+  saved_pred_Σ val ;
+  oneshot_Σ () () ;
+  mono_list_Σ gname ;
+  oneshot_Σ () () ;
+  mono_list_Σ gname
+].
+#[global] Instance subG_inf_mpmc_queue_2_Σ Σ `{zoo_G : !ZooG Σ} :
+  subG inf_mpmc_queue_2_Σ Σ →
+  InfMpmcQueue2G Σ.
+Proof.
+  solve_inG.
+Qed.
+
+Inductive ownership :=
+  | Own
+  | Discarded.
+
+Section inf_mpmc_queue_2_G.
+  Context `{inf_mpmc_queue_2_G : InfMpmcQueue2G Σ}.
+
+  Implicit Types Ψ : val → iProp Σ.
+
+  Record metadata := {
+    metadata_data : val ;
+    metadata_inv : namespace ;
+    metadata_prophet : gname ;
+    metadata_prophet_name : wise_prophets_name ;
+    metadata_front : gname ;
+    metadata_model : gname ;
+    metadata_history : gname ;
+    metadata_lstates : gname ;
+    metadata_producers : gname ;
+    metadata_consumers : gname ;
+  }.
+  Implicit Type γ : metadata.
+
+  #[local] Instance metadata_eq_dec : EqDecision metadata :=
+    ltac:(solve_decision).
+  #[local] Instance metadata_countable :
+    Countable metadata.
+  Proof.
+    solve_countable.
+  Qed.
+
+  #[local] Definition front_auth' γ_front i :=
+    auth_nat_max_auth γ_front (DfracOwn 1) i.
+  #[local] Definition front_auth γ i :=
+    front_auth' γ.(metadata_front) i.
+  #[local] Definition front_lb γ i :=
+    auth_nat_max_lb γ.(metadata_front) i.
+
+  #[local] Definition model₁' γ_model vs :=
+    twins_twin1 γ_model (DfracOwn 1) vs.
+  #[local] Definition model₁ γ vs :=
+    model₁' γ.(metadata_model) vs.
+  #[local] Definition model₂' γ_model vs :=
+    twins_twin2 γ_model vs.
+  #[local] Definition model₂ γ vs :=
+    model₂' γ.(metadata_model) vs.
+
+  #[local] Definition history_auth' γ_history hist :=
+    mono_list_auth γ_history (DfracOwn 1) hist.
+  #[local] Definition history_auth γ :=
+    history_auth' γ.(metadata_history).
+  #[local] Definition history_at γ i v :=
+    mono_list_at γ.(metadata_history) i (Some v).
+
+  #[local] Definition lstates_auth' γ_lstates lstates : iProp Σ :=
+    ∃ ηs,
+    mono_list_auth γ_lstates (DfracOwn 1) ηs ∗
+    [∗ list] η; lstate ∈ ηs; lstates,
+      auth_mono_auth _ η (DfracOwn 1) lstate.
+  #[local] Definition lstates_auth γ :=
+    lstates_auth' γ.(metadata_lstates).
+  #[local] Definition lstates_lb γ i lstate : iProp Σ :=
+    ∃ η,
+    mono_list_at γ.(metadata_lstates) i η ∗
+    auth_mono_lb _ η lstate.
+
+  #[local] Definition producers_auth' γ_producers i : iProp Σ :=
+    ∃ ηs,
+    mono_list_auth γ_producers (DfracOwn 1) ηs ∗
+    ⌜length ηs = i⌝.
+  #[local] Definition producers_auth γ :=
+    producers_auth' γ.(metadata_producers).
+  #[local] Definition producers_at γ i own : iProp Σ :=
+    ∃ η,
+    mono_list_at γ.(metadata_producers) i η ∗
+    match own with
+    | Own =>
+        oneshot_pending η (DfracOwn 1) ()
+    | Discarded =>
+        oneshot_shot η ()
+    end.
+
+  #[local] Definition consumers_auth' γ_consumers i : iProp Σ :=
+    ∃ ηs,
+    mono_list_auth γ_consumers (DfracOwn 1) ηs ∗
+    ⌜length ηs = i⌝.
+  #[local] Definition consumers_auth γ :=
+    consumers_auth' γ.(metadata_consumers).
+  #[local] Definition consumers_at γ i own : iProp Σ :=
+    ∃ η,
+    mono_list_at γ.(metadata_consumers) i η ∗
+    match own with
+    | Own =>
+        oneshot_pending η (DfracOwn 1) ()
+    | Discarded =>
+        oneshot_shot η ()
+    end.
+
+  #[local] Definition winner γ i : iProp Σ :=
+    ∃ id prophs,
+    wise_prophets_full prophet γ.(metadata_prophet_name) i prophs ∗
+    ⌜head prophs = Some id⌝ ∗
+    identifier_model' id.
+
+  #[local] Definition consumer_au γ Ψ : iProp Σ :=
+    AU <{
+      ∃∃ vs,
+      model₁ γ vs
+    }> @ ⊤ ∖ ↑γ.(metadata_inv), ∅ <{
+      ∀∀ v vs',
+      ⌜vs = v :: vs'⌝ ∗
+      model₁ γ vs'
+    , COMM
+      Ψ v
+    }>.
+
+  #[local] Definition inv_inner l γ : iProp Σ :=
+    ∃ slots front back vs hist lstates pasts prophss,
+    inf_array_model γ.(metadata_data) slots ∗
+    l.[front] ↦ #front ∗
+    l.[back] ↦ #back ∗
+    front_auth γ front ∗
+    model₂ γ vs ∗
+    ⌜vs = oflatten (drop front hist)⌝ ∗
+    history_auth γ hist ∗
+    ⌜length hist = back⌝ ∗
+    lstates_auth γ lstates ∗
+    ⌜length lstates = front `max` back⌝ ∗
+    wise_prophets_model prophet γ.(metadata_prophet) γ.(metadata_prophet_name) pasts prophss ∗
+    producers_auth γ back ∗
+    consumers_auth γ front ∗
+    ( [∗ list] i ↦ lstate ∈ take back lstates,
+      match lstate with
+      | ProducerProducer =>
+          winner γ i
+      | ProducerConsumer =>
+          True
+      | ConsumerProducer η =>
+          ∃ Ψ v,
+          front_lb γ i ∗
+          saved_pred η Ψ ∗
+          history_at γ i v ∗
+          Ψ v ∨ consumers_at γ i Discarded
+      | ConsumerConsumer =>
+          front_lb γ i
+      | _ =>
+          False
+      end
+    ) ∗
+    ( [∗ list] k ↦ lstate ∈ drop back lstates,
+      match lstate with
+      | ConsumerProducer η =>
+          ∃ Ψ,
+          saved_pred η Ψ ∗
+          consumer_au γ Ψ
+      | ConsumerConsumer =>
+          winner γ (back + k)
+      | _ =>
+          False
+      end
+    ) ∗
+    ( ∀ i,
+      match slots i with
+      | Nothing =>
+          ⌜pasts i = []⌝
+      | Something v =>
+          history_at γ i v ∗
+          lstates_lb γ i Producer ∗
+          producers_at γ i Discarded
+      | Anything =>
+          lstates_lb γ i Consumer ∗
+          consumers_at γ i Discarded
+      end
+    ).
+  Definition inf_mpmc_queue_2_inv t ι : iProp Σ :=
+    ∃ l γ,
+    ⌜t = #l⌝ ∗
+    meta l nroot γ ∗
+    l.[data] ↦□ γ.(metadata_data) ∗
+    inf_array_inv γ.(metadata_data) ∗
+    inv ι (inv_inner l γ).
+
+  Definition inf_mpmc_queue_2_model t vs : iProp Σ :=
+    ∃ l γ,
+    ⌜t = #l⌝ ∗
+    meta l nroot γ ∗
+    model₁ γ vs.
+
+  Opaque lstates_auth'.
+  Opaque lstates_lb.
+  Opaque producers_auth'.
+  Opaque producers_at.
+  Opaque consumers_auth'.
+  Opaque consumers_at.
+
+  Lemma inf_mpmc_queue_2_create_spec ι :
+    {{{
+      True
+    }}}
+      inf_mpmc_queue_2_create ()
+    {{{ t,
+      RET t;
+      inf_mpmc_queue_2_inv t ι ∗
+      inf_mpmc_queue_2_model t []
+    }}}.
+  Proof.
+  Admitted.
+
+  Lemma inf_mpmc_queue_2_size_spec t ι :
+    <<<
+      inf_mpmc_queue_2_inv t ι
+    | ∀∀ vs,
+      inf_mpmc_queue_2_model t vs
+    >>>
+      inf_mpmc_queue_2_size t @ ↑ι
+    <<<
+      inf_mpmc_queue_2_model t vs
+    | RET #(length vs);
+      True
+    >>>.
+  Proof.
+  Admitted.
+
+  Lemma inf_mpmc_queue_2_is_empty_spec t ι :
+    <<<
+      inf_mpmc_queue_2_inv t ι
+    | ∀∀ vs,
+      inf_mpmc_queue_2_model t vs
+    >>>
+      inf_mpmc_queue_2_is_empty t @ ↑ι
+    <<<
+      inf_mpmc_queue_2_model t vs
+    | RET #(bool_decide (vs = []%list));
+      True
+    >>>.
+  Proof.
+  Admitted.
+
+  Lemma inf_mpmc_queue_2_push_spec t ι v :
+    <<<
+      inf_mpmc_queue_2_inv t ι
+    | ∀∀ vs,
+      inf_mpmc_queue_2_model t vs
+    >>>
+      inf_mpmc_queue_2_push t v @ ↑ι
+    <<<
+      inf_mpmc_queue_2_model t (vs ++ [v])
+    | RET ();
+      True
+    >>>.
+  Proof.
+  Admitted.
+
+  Lemma inf_mpmc_queue_2_pop_spec t ι :
+    <<<
+      inf_mpmc_queue_2_inv t ι
+    | ∀∀ vs,
+      inf_mpmc_queue_2_model t vs
+    >>>
+      inf_mpmc_queue_2_pop t @ ↑ι
+    <<<
+      ∃∃ v vs',
+      ⌜vs = v :: vs'⌝ ∗
+      inf_mpmc_queue_2_model t vs'
+    | RET v;
+      True
+    >>>.
+  Proof.
+  Admitted.
+End inf_mpmc_queue_2_G.
+
 #[global] Opaque inf_mpmc_queue_2_create.
 #[global] Opaque inf_mpmc_queue_2_size.
 #[global] Opaque inf_mpmc_queue_2_is_empty.
 #[global] Opaque inf_mpmc_queue_2_push.
 #[global] Opaque inf_mpmc_queue_2_pop.
+
+#[global] Opaque inf_mpmc_queue_2_inv.
+#[global] Opaque inf_mpmc_queue_2_model.
